src/Database/Common.v
@@ -1,7 +1,7 @@
 From RecoveryRefinement Require Export Helpers.MachinePrimitives.
 From RecoveryRefinement Require Export Database.DataStructures.
 
-Definition Key := int64.
+Definition Key := uint64.
 Definition Value := ByteString.
 
 Module Entry.
@@ -12,6 +12,6 @@ End Entry.
 
 Module SliceHandle.
   Record t :=
-    mk { offset : int64;
-         length : int32; }.
+    mk { offset : uint64;
+         length : uint32; }.
 End SliceHandle.
